theories/tree_prop.v
@@ -417,8 +417,8 @@ Section RunP.
       same_structure_sup A (dead A).
     Proof. case: A => //=. Qed.
 
-    Lemma runb_same_structure {s A s1 r n}:
-      runb u s A s1 r n -> same_structure_sup A r.
+    Lemma run_same_structure {s A s1 r n}:
+      run u s A s1 r n -> same_structure_sup A r.
     Proof.
       elim; clear => //.
       - move=> s1 s2 A B sA _ <-/=.
@@ -437,7 +437,7 @@ Section RunP.
     Qed.
 
     Lemma run_dead1 {s1 B s2 r n}:  
-      is_dead B -> runb u s1 B s2 r n -> (s2 = None /\ r = dead B /\ n = false)%type2.
+      is_dead B -> run u s1 B s2 r n -> (s2 = None /\ r = dead B /\ n = false)%type2.
     Proof.
       move=> dB H; inversion H; clear H; subst;
         try rewrite // is_dead_step//is_dead_dead in H0.
@@ -446,7 +446,7 @@ Section RunP.
     Qed.
 
     Lemma run_dead2 {s1 B s2 r n}:  
-      runb u s1 (dead B) s2 r n -> (s2 = None /\ r = dead B /\ n = false)%type2.
+      run u s1 (dead B) s2 r n -> (s2 = None /\ r = dead B /\ n = false)%type2.
     Proof. move=> /(run_dead1 is_dead_dead)//; rewrite dead2//. Qed.
 
   End same_structure.
@@ -504,7 +504,7 @@ Section RunP.
     next_alt false (big_and p r) = Some (big_and p r).
   Proof. elim: r p => //=x xs IH p; case: x => //=. Qed.
 
-  Lemma is_ko_runb {s A}: is_ko A -> runb u s A None (dead A) false.
+  Lemma is_ko_run {s A}: is_ko A -> run u s A None (dead A) false.
   Proof.
     elim: A s => //=.
     - by move=> s _; apply: run_dead => //=.
@@ -522,26 +522,26 @@ Section RunP.
       by rewrite is_ko_success//=is_ko_failed//is_ko_next_alt//.
   Qed.
 
-  Lemma runb_success1 {A} s: 
-    success A -> runb u s A (Some (get_substS s A)) (build_na A (next_alt true A)) false.
+  Lemma run_success1 {A} s: 
+    success A -> run u s A (Some (get_substS s A)) (build_na A (next_alt true A)) false.
   Proof.
     move=> sA.
     by apply: run_done.
   Qed.
 
-  Lemma runb_success {A s1 s2 r n}: 
-    success A -> runb u s1 A s2 r n -> (s2 = Some (get_substS s1 A) /\ r = build_na A (next_alt true A) /\ n = false)%type2.
+  Lemma run_success {A s1 s2 r n}: 
+    success A -> run u s1 A s2 r n -> (s2 = Some (get_substS s1 A) /\ r = build_na A (next_alt true A) /\ n = false)%type2.
   Proof.
     move=> sA H; have:= succes_step s1 sA.
     by inversion H; clear H; try congruence; subst; rewrite succes_step//; rewrite failed_success in sA.
   Qed.
 
   Lemma run_consistent {s A s1 B s2 C n1 n2}:
-    runb u s A s1 B n1 -> runb u s A s2 C n2 -> ((s2 = s1) /\ (C = B) /\ (n2 = n1))%type2.
+    run u s A s1 B n1 -> run u s A s2 C n2 -> ((s2 = s1) /\ (C = B) /\ (n2 = n1))%type2.
   Proof.
     move=> H; elim: H s2 C n2; clear.
     + move=> s1 _ A _ sA <-<- s3 C n2 H; subst.
-      by apply: runb_success sA H.
+      by apply: run_success sA H.
     + move=> s1 s2 r A B n1 HA HB IH s4 r' n2 H.
       inversion H; clear H; try congruence; subst.
       - by rewrite succes_step in HA.
