theories/tree_valid_state.v
@@ -343,7 +343,7 @@ Section valid_tree.
     Qed.
 
   Lemma valid_tree_run {s1 A s2 B b}:
-    valid_tree A -> runb u s1 A s2 B b -> (B = dead B) + valid_tree B.
+    valid_tree A -> run u s1 A s2 B b -> (B = dead B) + valid_tree B.
   Proof.
     move=> + H; elim: H; clear => //=.
     + move=> s1 s2 A B sA _ <- vA.
